src/Std/Data/Iterators/TempLawfulMonadLift.lean
@@ -5,6 +5,7 @@ Authors: Quang Dao
 -/
 prelude
 import Init.Control.Basic
+import Init.Control.Lawful.Basic
 
 /-!
 # LawfulMonadLift and LawfulMonadLiftT
@@ -48,3 +49,97 @@ class LawfulMonadLiftT (m : Type u → Type v) (n : Type u → Type w) [Monad m]
 export LawfulMonadLiftT (monadLift_pure monadLift_bind)
 
 end MonadLift
+
+section Lemmas
+universe u v w
+
+variable {m : Type u → Type v} {n : Type u → Type w} [Monad m] [Monad n] [MonadLiftT m n]
+  [LawfulMonadLiftT m n] {α β : Type u}
+
+theorem monadLift_map [LawfulMonad m] [LawfulMonad n] (f : α → β) (ma : m α) :
+    monadLift (f <$> ma) = f <$> (monadLift ma : n α) := by
+  rw [← bind_pure_comp, ← bind_pure_comp, monadLift_bind]
+  simp only [bind_pure_comp, monadLift_pure]
+
+theorem monadLift_seq [LawfulMonad m] [LawfulMonad n] (mf : m (α → β)) (ma : m α) :
+    monadLift (mf <*> ma) = monadLift mf <*> (monadLift ma : n α) := by
+  simp only [seq_eq_bind, monadLift_map, monadLift_bind]
+
+theorem monadLift_seqLeft [LawfulMonad m] [LawfulMonad n] (x : m α) (y : m β) :
+    monadLift (x <* y) = (monadLift x : n α) <* (monadLift y : n β) := by
+  simp only [seqLeft_eq, monadLift_map, monadLift_seq]
+
+theorem monadLift_seqRight [LawfulMonad m] [LawfulMonad n] (x : m α) (y : m β) :
+    monadLift (x *> y) = (monadLift x : n α) *> (monadLift y : n β) := by
+  simp only [seqRight_eq, monadLift_map, monadLift_seq]
+
+/-! We duplicate the theorems for `monadLift` to `liftM` since `rw` matches on syntax only. -/
+
+@[simp]
+theorem liftM_pure (a : α) : liftM (pure a : m α) = pure (f := n) a :=
+  monadLift_pure _
+
+@[simp]
+theorem liftM_bind (ma : m α) (f : α → m β) :
+    liftM (n := n) (ma >>= f) = liftM ma >>= (fun a => liftM (f a)) :=
+  monadLift_bind _ _
+
+@[simp]
+theorem liftM_map [LawfulMonad m] [LawfulMonad n] (f : α → β) (ma : m α) :
+    liftM (f <$> ma) = f <$> (liftM ma : n α) :=
+  monadLift_map _ _
+
+@[simp]
+theorem liftM_seq [LawfulMonad m] [LawfulMonad n] (mf : m (α → β)) (ma : m α) :
+    liftM (mf <*> ma) = liftM mf <*> (liftM ma : n α) :=
+  monadLift_seq _ _
+
+@[simp]
+theorem liftM_seqLeft [LawfulMonad m] [LawfulMonad n] (x : m α) (y : m β) :
+    liftM (x <* y) = (liftM x : n α) <* (liftM y : n β) :=
+  monadLift_seqLeft _ _
+
+@[simp]
+theorem liftM_seqRight [LawfulMonad m] [LawfulMonad n] (x : m α) (y : m β) :
+    liftM (x *> y) = (liftM x : n α) *> (liftM y : n β) :=
+  monadLift_seqRight _ _
+
+end Lemmas
+
+section MonadLiftFunction
+
+class LawfulMonadLiftFunction {m : Type u → Type v} {n : Type u → Type w}
+    [Monad m] [Monad n] (lift : ⦃α : Type u⦄ → m α → n α) where
+  lift_pure {α : Type u} (a : α) : lift (pure a) = pure a
+  lift_bind {α β : Type u} (ma : m α) (f : α → m β) :
+    lift (ma >>= f) = lift ma >>= (fun x => lift (f x))
+
+instance {m : Type u → Type v} [Monad m] : LawfulMonadLiftFunction (fun ⦃α⦄ => (id : m α → m α)) where
+  lift_pure := by simp
+  lift_bind := by simp
+
+variable {m : Type u → Type v} {n : Type u → Type w} [Monad m] [Monad n]
+    {lift : ⦃α : Type u⦄ → m α → n α}
+
+theorem LawfulMonadLiftFunction.lift_map [LawfulMonad m] [LawfulMonad n]
+    [LawfulMonadLiftFunction lift] (f : α → β) (ma : m α) :
+    lift (f <$> ma) = f <$> (lift ma : n α) := by
+  rw [← bind_pure_comp, ← bind_pure_comp, lift_bind (lift := lift)]
+  simp only [bind_pure_comp, lift_pure]
+
+theorem LawfulMonadLiftFunction.lift_seq [LawfulMonad m] [LawfulMonad n]
+    [LawfulMonadLiftFunction lift] (mf : m (α → β)) (ma : m α) :
+    lift (mf <*> ma) = lift mf <*> (lift ma : n α) := by
+  simp only [seq_eq_bind, lift_map, lift_bind]
+
+theorem LawfulMonadLiftFunction.lift_seqLeft [LawfulMonad m] [LawfulMonad n]
+    [LawfulMonadLiftFunction lift] (x : m α) (y : m β) :
+    lift (x <* y) = (lift x : n α) <* (lift y : n β) := by
+  simp only [seqLeft_eq, lift_map, lift_seq]
+
+theorem LawfulMonadLiftFunction.lift_seqRight [LawfulMonad m] [LawfulMonad n]
+    [LawfulMonadLiftFunction lift] (x : m α) (y : m β) :
+    lift (x *> y) = (lift x : n α) *> (lift y : n β) := by
+  simp only [seqRight_eq, lift_map, lift_seq]
+
+end MonadLiftFunction
