src/Std/Data/Iterators/Lemmas/Consumers/Monadic/Loop.lean
@@ -130,7 +130,7 @@ theorem IterM.fold_eq_match_step {α β γ : Type w} {m : Type w → Type w'} [I
 
 theorem IterM.toList_eq_fold {α β : Type w} {m : Type w → Type w'} [Iterator α m β]
     [Finite α m] [Monad m] [LawfulMonad m] [IteratorLoop α m m] [LawfulIteratorLoop α m m]
-    [IteratorCollect α m] [LawfulIteratorCollect α m]
+    [IteratorCollect α m m] [LawfulIteratorCollect α m m]
     {it : IterM (α := α) m β} :
     it.toList = it.fold (init := []) (fun l out => l ++ [out]) := by
   suffices h : ∀ l' : List β, (l' ++ ·) <$> it.toList =
@@ -179,7 +179,7 @@ theorem IterM.drain_eq_match_step {α β : Type w} {m : Type w → Type w'} [Ite
 
 theorem IterM.drain_eq_map_toList {α β : Type w} {m : Type w → Type w'} [Iterator α m β]
     [Finite α m] [Monad m] [LawfulMonad m] [IteratorLoop α m m] [LawfulIteratorLoop α m m]
-    [IteratorCollect α m] [LawfulIteratorCollect α m]
+    [IteratorCollect α m m] [LawfulIteratorCollect α m m]
     {it : IterM (α := α) m β} :
     it.drain = (fun _ => .unit) <$> it.toList := by
   induction it using IterM.inductSteps with | step it ihy ihs =>
@@ -196,14 +196,14 @@ theorem IterM.drain_eq_map_toList {α β : Type w} {m : Type w → Type w'} [Ite
 
 theorem IterM.drain_eq_map_toListRev {α β : Type w} {m : Type w → Type w'} [Iterator α m β]
     [Finite α m] [Monad m] [LawfulMonad m] [IteratorLoop α m m] [LawfulIteratorLoop α m m]
-    [IteratorCollect α m] [LawfulIteratorCollect α m]
+    [IteratorCollect α m m] [LawfulIteratorCollect α m m]
     {it : IterM (α := α) m β} :
     it.drain = (fun _ => .unit) <$> it.toListRev := by
   simp [IterM.drain_eq_map_toList, IterM.toListRev_eq]
 
 theorem IterM.drain_eq_map_toArray {α β : Type w} {m : Type w → Type w'} [Iterator α m β]
     [Finite α m] [Monad m] [LawfulMonad m] [IteratorLoop α m m] [LawfulIteratorLoop α m m]
-    [IteratorCollect α m] [LawfulIteratorCollect α m]
+    [IteratorCollect α m m] [LawfulIteratorCollect α m m]
     {it : IterM (α := α) m β} :
     it.drain = (fun _ => .unit) <$> it.toList := by
   simp [IterM.drain_eq_map_toList]
